add refinement proof using MITL specifications

semantics/mitlScript.sml
@@ -346,4 +346,222 @@ Definition mitl_example:
   (mitl_box (interval_right_half_open_inf 0) (mitl_const b))
 End
 
+(* []_[0,inf) (P0 -> <->_[0,t] P1) *)
+Definition mitl_always_occ_past_def:
+ mitl_always_occ_past (P0 : 'a) (P1 : 'a) (t : num) : 'a f =
+  (mitl_box
+   (interval_right_half_open_inf 0)
+   (mitl_implies 
+    (mitl_const P0)
+    (mitl_diamond_dash (interval_closed 0 t) (mitl_const P1))))
+End
+
+(* .... *)
+
+Theorem num_le_minus[local]:
+ !(x:num) (y:num) (z:num). x <= z /\ z - 0 <= y /\ y <= z ==> x <= y
+Proof
+ rw [] >> DECIDE_TAC
+QED
+
+Theorem timed_word_wf_lt_pos_shift_interval_right_half_open_inf_zero:
+ !(tau:'a timed_word). (!i j. i < j ==> (SND (tau i)) < (SND (tau j))) ==>
+  !i j.
+  SND (tau i) IN interval_pos_shift (SND (tau j)) (interval_right_half_open_inf 0) ==>
+  j <= i
+Proof
+ rw [interval_pos_shift] >>
+ Cases_on `i < j` >-
+  (`SND (tau i) < SND (tau j)` by METIS_TAC [] >>
+   METIS_TAC [REAL_LET_ANTISYM]) >>
+ DECIDE_TAC
+QED
+
+Theorem timed_word_wf_lt_neg_shift_interval_closed_zero:
+ !(tau:'a timed_word). (!i j. i < j ==> (SND (tau i)) < (SND (tau j))) ==>
+  !i j t.
+  SND (tau i) IN interval_neg_shift (SND (tau j)) (interval_closed 0 t) ==>
+  i <= j
+Proof
+ rw [interval_neg_shift] >>
+ Cases_on `j < i` >-
+  (`SND (tau j) < SND (tau i)` by METIS_TAC [] >>
+   METIS_TAC [REAL_LET_ANTISYM]) >>
+ DECIDE_TAC
+QED
+
+Theorem mitl_pos_neg_shift_right_open_inf:
+ !(tau:'a timed_word). SND (tau 0) = 0 ==>
+  !i j t.
+  SND (tau i) IN interval_pos_shift (SND (tau 0)) (interval_right_half_open_inf 0) /\
+  SND (tau j) IN interval_neg_shift (SND (tau i)) (interval_closed 0 t) ==>
+  SND (tau j) IN interval_pos_shift (SND (tau 0)) (interval_right_half_open_inf 0)
+Proof
+ rw [interval_pos_shift,interval_neg_shift] >>
+ fs [real_ge]
+QED
+
+Theorem real_to_num_plus_le[local]:
+ !x y z t0 t1. 
+ x >= 0 /\
+ y - &t0 <= x /\
+ x <= y /\
+ z >= 0 /\
+ x - &t1 <= z /\
+ z ≤ x ==>
+ y - (&t0 + &t1) <= z
+Proof
+ rw [] >>
+ once_rewrite_tac [GSYM REAL_OF_NUM_ADD] >>
+ `&t0 >= 0` by REAL_ARITH_TAC >>
+ `&t1 >= 0` by REAL_ARITH_TAC >>
+ `x - &t1 <= x` by REAL_ARITH_TAC >>
+ `y - (&t0 + &t1) <= y - &t0` by REAL_ARITH_TAC >>
+ `(y - &t0) - &t1 <= z` suffices_by REAL_ARITH_TAC >>
+ `y - &t0 - &t1 <= x - &t1` suffices_by METIS_TAC [REAL_LE_TRANS] >>
+ METIS_TAC [REAL_LE_SUB_CANCEL2]
+QED
+
+Theorem mitl_neg_shift_interval_closed_plus:
+ !(tau:'a timed_word).
+  !i j k t0 t1.
+  SND (tau j) IN interval_neg_shift (SND (tau i)) (interval_closed 0 t0) /\
+  SND (tau k) IN interval_neg_shift (SND (tau j)) (interval_closed 0 t1) ==>
+  SND (tau k) IN interval_neg_shift (SND (tau i)) (interval_closed 0 (t0 + t1))
+Proof
+ rw [interval_neg_shift] >-
+  (once_rewrite_tac [GSYM REAL_OF_NUM_ADD] >>
+   METIS_TAC [real_to_num_plus_le]) >>  
+ METIS_TAC [REAL_LE_TRANS]
+QED
+
+Theorem mitl_always_occ_past_two:
+ !(tau:'a timed_word). SND (tau 0) = 0 ==>
+ !state_holds P0 P1 P2 t0 t1.
+  mitl_general_holds state_holds tau 0 (mitl_always_occ_past P0 P1 t0) /\
+  mitl_general_holds state_holds tau 0 (mitl_always_occ_past P1 P2 t1) ==>
+  mitl_general_holds state_holds tau 0 (mitl_always_occ_past P0 P2 (t0+t1))
+Proof
+ rw [mitl_always_occ_past_def] >>
+ fs [mitl_general_holds] >> 
+ rw [] >>
+ `?j'. SND (tau j') IN interval_neg_shift (SND (tau j)) (interval_closed 0 t0) /\ state_holds (FST (tau j')) P1`
+  by METIS_TAC [] >>
+
+ `SND (tau j') IN interval_pos_shift (SND (tau 0)) (interval_right_half_open_inf 0)`
+  by METIS_TAC [mitl_pos_neg_shift_right_open_inf] >>
+
+ `?j''. SND (tau j'') IN interval_neg_shift (SND (tau j')) (interval_closed 0 t1) /\ state_holds (FST (tau j'')) P2`
+  by METIS_TAC [] >>
+ 
+ Q.EXISTS_TAC `j''` >> rw [] >>
+
+ METIS_TAC [mitl_neg_shift_interval_closed_plus]
+QED
+
+Theorem real_to_num_plus_le_three[local]:
+ !x y z a t0 t1 t2.  
+ x ≥ 0 /\
+ y − &t0 ≤ x /\
+ x ≤ y /\
+ z ≥ 0 /\
+ x − &t1 ≤ z /\
+ z ≤ x /\
+ a ≥ 0 /\
+ z − &t2 ≤ a /\
+ a ≤ z ==>
+ y − (&t0 + &t1 + &t2) ≤ a
+Proof
+ rw [] >>
+ once_rewrite_tac [GSYM REAL_OF_NUM_ADD] >>
+ once_rewrite_tac [GSYM REAL_OF_NUM_ADD] >>
+ once_rewrite_tac [REAL_ADD_ASSOC] >>
+ `&t0 >= 0` by REAL_ARITH_TAC >>
+ `&t1 >= 0` by REAL_ARITH_TAC >>
+ `&t2 >= 0` by REAL_ARITH_TAC >>
+
+ `x - &t1 <= x` by REAL_ARITH_TAC >>
+ `y - (&t0 + &t1) <= y - &t0` by REAL_ARITH_TAC >>
+
+ `y - (&t0 + &t1 + &t2) <= y - &t0` by REAL_ARITH_TAC >>
+
+ `y - &t0 - &t1 - &t2 ≤ a` suffices_by REAL_ARITH_TAC >>
+ 
+ `y - &t0 - &t1 - &t2 <= z - &t2` suffices_by METIS_TAC [REAL_LE_TRANS] >>
+ 
+ `y - &t0 - &t1 <= z` suffices_by METIS_TAC [REAL_LE_SUB_CANCEL2] >>
+
+ `y - &t0 - &t1 <= x - &t1` suffices_by METIS_TAC [REAL_LE_TRANS] >>
+
+ METIS_TAC [REAL_LE_SUB_CANCEL2]
+QED
+
+Theorem mitl_neg_shift_interval_closed_plus_three:
+ !(tau:'a timed_word).
+  !i j k l t0 t1 t2.
+  SND (tau j) IN interval_neg_shift (SND (tau i)) (interval_closed 0 t0) /\
+  SND (tau k) IN interval_neg_shift (SND (tau j)) (interval_closed 0 t1) /\
+  SND (tau l) IN interval_neg_shift (SND (tau k)) (interval_closed 0 t2) ==>  
+  SND (tau l) IN interval_neg_shift (SND (tau i)) (interval_closed 0 (t0 + (t1 + t2)))
+Proof
+ rw [interval_neg_shift] >-
+  (once_rewrite_tac [GSYM REAL_OF_NUM_ADD] >>
+   once_rewrite_tac [GSYM REAL_OF_NUM_ADD] >>
+   once_rewrite_tac [REAL_ADD_ASSOC] >>   
+   METIS_TAC [real_to_num_plus_le_three]) >>  
+ METIS_TAC [REAL_LE_TRANS]
+QED
+
+Theorem mitl_always_occ_past_three:
+ !(tau:'a timed_word). SND (tau 0) = 0 ==>
+ !state_holds P0 P1 P2 P3 t0 t1 t2.
+  mitl_general_holds state_holds tau 0 (mitl_always_occ_past P0 P1 t0) /\
+  mitl_general_holds state_holds tau 0 (mitl_always_occ_past P1 P2 t1) /\
+  mitl_general_holds state_holds tau 0 (mitl_always_occ_past P2 P3 t2) ==>
+  mitl_general_holds state_holds tau 0 (mitl_always_occ_past P0 P3 (t0+t1+t2))
+Proof
+ rw [mitl_always_occ_past_def] >>
+ fs [mitl_general_holds] >> 
+ rw [] >>
+ `?j'. SND (tau j') IN interval_neg_shift (SND (tau j)) (interval_closed 0 t0) /\ state_holds (FST (tau j')) P1`
+  by METIS_TAC [] >>
+
+ `SND (tau j') IN interval_pos_shift (SND (tau 0)) (interval_right_half_open_inf 0)`
+  by METIS_TAC [mitl_pos_neg_shift_right_open_inf] >>
+
+ `?j''. SND (tau j'') IN interval_neg_shift (SND (tau j')) (interval_closed 0 t1) /\ state_holds (FST (tau j'')) P2`
+  by METIS_TAC [] >>
+
+ `SND (tau j'') IN interval_pos_shift (SND (tau 0)) (interval_right_half_open_inf 0)`
+  by METIS_TAC [mitl_pos_neg_shift_right_open_inf] >>
+
+ `?j'''. SND (tau j''') IN interval_neg_shift (SND (tau j'')) (interval_closed 0 t2) /\ state_holds (FST (tau j''')) P3`
+  by METIS_TAC [] >>
+ 
+ Q.EXISTS_TAC `j'''` >> rw [] >>
+
+ METIS_TAC [mitl_neg_shift_interval_closed_plus_three]
+QED
+
+Theorem mitl_sem_always_occ_past_three:
+ !(tau:'a timed_word). SND (tau 0) = 0 ==>
+ !omega. (!i. timed_word_suffix tau i IN omega) ==>
+ !state_holds P0 P1 P2 P3 t0 t1 t2.
+   tau IN mitl_general_sem state_holds omega 0 (mitl_always_occ_past P0 P1 t0) /\
+   tau IN mitl_general_sem state_holds omega 0 (mitl_always_occ_past P1 P2 t1) /\
+   tau IN mitl_general_sem state_holds omega 0 (mitl_always_occ_past P2 P3 t2) ==>
+   tau IN mitl_general_sem state_holds omega 0 (mitl_always_occ_past P0 P3 (t0+t1+t2))
+Proof
+ REPEAT STRIP_TAC >>
+ `mitl_general_holds state_holds tau 0 (mitl_always_occ_past P0 P1 t0)`
+  by METIS_TAC [mitl_general_holds_sem] >>
+ `mitl_general_holds state_holds tau 0 (mitl_always_occ_past P1 P2 t1)`
+  by METIS_TAC [mitl_general_holds_sem] >>
+ `mitl_general_holds state_holds tau 0 (mitl_always_occ_past P2 P3 t2)`
+  by METIS_TAC [mitl_general_holds_sem] >>
+ `mitl_general_holds state_holds tau 0 (mitl_always_occ_past P0 P3 (t0+t1+t2))`
+  suffices_by METIS_TAC [mitl_general_holds_sem] >>
+ METIS_TAC [mitl_always_occ_past_three]
+QED
+
 val _ = export_theory ();
