semantics/compSpecMitlScript.sml
@@ -130,4 +130,90 @@ Proof
  ]
 QED
 
+Theorem St_sem_double_par_intersection1:
+ !state_holds omega MS MV S1 S2 S3 x. 
+  x IN St_sem state_holds omega MS MV (St_par S1 (St_par S2 S3)) ==>
+  x IN { a INTER b INTER c | a IN St_sem state_holds omega MS MV S1 /\
+     b IN St_sem state_holds omega MS MV S2 /\ c IN St_sem state_holds omega MS MV S3 }
+Proof
+ rw [St_sem,double_intersection] >>
+ Q.EXISTS_TAC `a` >>
+ Q.EXISTS_TAC `a'` >>
+ Q.EXISTS_TAC `b'` >>
+ rw [] >> 
+ METIS_TAC [INTER_ASSOC]
+QED
+
+Theorem St_sem_double_par_intersection2:
+ !state_holds omega MS MV S1 S2 S3 x. 
+  x IN { a INTER b INTER c | a IN St_sem state_holds omega MS MV S1 /\
+     b IN St_sem state_holds omega MS MV S2 /\ c IN St_sem state_holds omega MS MV S3 } ==>
+  x IN St_sem state_holds omega MS MV (St_par S1 (St_par S2 S3))
+Proof
+ rw [St_sem,double_intersection] >>
+ Q.EXISTS_TAC `a` >>
+ Q.EXISTS_TAC `b INTER c` >>
+ rw [] >- METIS_TAC [INTER_ASSOC] >>
+ Q.EXISTS_TAC `b` >>
+ Q.EXISTS_TAC `c` >>
+ rw []
+QED
+
+Theorem St_sem_double_par_intersection:
+ !state_holds omega MS MV S1 S2 S3. 
+  St_sem state_holds omega MS MV (St_par S1 (St_par S2 S3)) =
+   { a INTER b INTER c | a IN St_sem state_holds omega MS MV S1 /\
+     b IN St_sem state_holds omega MS MV S2 /\ c IN St_sem state_holds omega MS MV S3 }
+Proof
+ rw [] >>
+ once_rewrite_tac [EXTENSION] >>
+ METIS_TAC [St_sem_double_par_intersection1,St_sem_double_par_intersection2]
+QED
+
+Theorem Pt_sem_mitl_sem_always_occ_past_three:
+ !state_holds omega Mc MS Mq MV P0 P1 P2 P3 t0 t1 t2.
+ (!tau. tau IN omega ==> SND (tau 0) = 0 /\ !i. timed_word_suffix tau i IN omega) ==>
+ Pt_sem state_holds omega Mc MS Mq MV
+  (Pt_refines 
+   (St_par (St_const (T_hat (mitl_always_occ_past P0 P1 t0)))
+     (St_par (St_const (T_hat (mitl_always_occ_past P1 P2 t1))) (St_const (T_hat (mitl_always_occ_past P2 P3 t2)))))
+   (St_const (T_hat (mitl_always_occ_past P0 P3 (t0+t1+t2)))))
+Proof
+ rw [Pt_sem,St_sem_double_par_intersection,St_sem,SUBSET_DEF] >>
+ `t0 + (t1 + t2) = t0 + t1 + t2` by rw [REAL_ADD_ASSOC] >>
+ `a ∩ b ∩ c SUBSET (mitl_general_sem state_holds omega 0 (mitl_always_occ_past P0 P3 (t0 + t1 + t2)))`
+  suffices_by METIS_TAC [IN_POW] >>
+
+ `a SUBSET (mitl_general_sem state_holds omega 0 (mitl_always_occ_past P0 P1 t0))`
+  by METIS_TAC [IN_POW] >>
+
+ `b SUBSET (mitl_general_sem state_holds omega 0 (mitl_always_occ_past P1 P2 t1))`
+  by METIS_TAC [IN_POW] >>
+
+ `c SUBSET (mitl_general_sem state_holds omega 0 (mitl_always_occ_past P2 P3 t2))`
+  by METIS_TAC [IN_POW] >>
+
+ fs [SUBSET_DEF,INTER_DEF] >>
+
+ rw [] >>
+
+ `x IN mitl_general_sem state_holds omega 0 (mitl_always_occ_past P0 P1 t0)`
+  by METIS_TAC [] >>
+
+ `x IN mitl_general_sem state_holds omega 0 (mitl_always_occ_past P1 P2 t1)`
+  by METIS_TAC [] >>
+
+ `x IN mitl_general_sem state_holds omega 0 (mitl_always_occ_past P2 P3 t2)`
+  by METIS_TAC [] >>
+
+ `t0 + (t1 + t2) = t0 + t1 + t2` by rw [REAL_ADD_ASSOC] >>
+
+ `x IN mitl_general_sem state_holds omega 0 (mitl_always_occ_past P0 P3 (t0 + t1 + t2))`
+  suffices_by METIS_TAC [] >>
+
+ `x IN omega` suffices_by METIS_TAC [mitl_sem_always_occ_past_three] >>
+
+ METIS_TAC [mitl_general_sem_omega,SUBSET_DEF]
+QED
+
 val _ = export_theory ();
